Add predicate "is zero" and binary relation "are equal" to Church numeral theory.  Proof that the latter works is disgusting.  Will need to develop some better technology here.  Thomas Tuerk's congLib is probably the way to go.  Minor additions to Church booleans, and a new theory of Church pairs, showing only that fst (pair x y) = x and snd (pair x y) = y.  Not sure what else is possible.

examples/lambda/computability/churchnumScript.sml
@@ -5,15 +5,13 @@ open pred_setTheory
 open termTheory
 open boolSimps
 open normal_orderTheory
+open churchboolTheory
+
+fun Store_thm(n,t,tac) = store_thm(n,t,tac) before export_rewrites [n]
 
 val _ = new_theory "churchnum"
 
 val _ = set_trace "Unicode" 1
-
-val _ = remove_ovl_mapping "LAM" {Name="LAM", Thy="labelledTerms"}
-val _ = remove_ovl_mapping "FV"  {Name="FV",  Thy="labelledTerms"}
-val _ = remove_ovl_mapping "VAR" {Name="VAR", Thy="labelledTerms"}
-val _ = remove_ovl_mapping "@@"  {Name="APP", Thy="labelledTerms"}
 
 val church_def = Define`
   church n = LAM "z" (LAM "s" (FUNPOW ((@@) (VAR "s")) n (VAR "z")))
@@ -43,6 +41,11 @@ val bnf_church = store_thm(
   Induct_on `n` THEN SRW_TAC [][] THEN
   SRW_TAC [][FUNPOW_SUC]);
 val _ = export_rewrites ["bnf_church"]
+
+val is_abs_church = Store_thm(
+  "is_abs_church",
+  ``is_abs (church n)``,
+  SRW_TAC [][church_def]);
 
 val church_lameq_11 = store_thm(
   "church_lameq_11",
@@ -275,6 +278,11 @@ val cpred_bnf = store_thm(
   SRW_TAC [][cpred_def, normorder_rwts]);
 val _ = export_rewrites ["cpred_bnf"]
 
+val bnf_cpred = Store_thm(
+  "bnf_cpred",
+  ``bnf cpred``,
+  SRW_TAC [][cpred_def]);
+
 val FV_cpred = store_thm(
   "FV_cpred",
   ``FV cpred = {}``,
@@ -434,6 +442,120 @@ val cmult_behaviour = store_thm(
   Q.EXISTS_TAC `cplus @@ church n @@ church (m * n)` THEN
   SRW_TAC [][betastar_APPr, nstar_betastar, arithmeticTheory.MULT_CLAUSES] THEN
   METIS_TAC [nstar_betastar, cplus_behaviour, arithmeticTheory.ADD_COMM])
+
+(* predicates/relations *)
+val cis_zero_def = Define`
+  cis_zero = LAM "n" (VAR "n" @@ cB T @@ (LAM "x" (cB F)))
+`;
+val FV_cis_zero = Store_thm(
+  "FV_cis_zero",
+  ``FV cis_zero = {}``,
+  SRW_TAC [][cis_zero_def, EXTENSION]);
+val bnf_cis_zero = Store_thm(
+  "bnf_cis_zero",
+  ``bnf cis_zero``,
+  SRW_TAC [][cis_zero_def]);
+
+val cis_zero_behaviour = store_thm(
+  "cis_zero_behaviour",
+  ``cis_zero @@ church n -n->* cB (n = 0)``,
+  Cases_on `n = 0` THEN SRW_TAC [][cis_zero_def] THEN
+  SRW_TAC [][Once relationTheory.RTC_CASES1, normorder_rwts, lemma14b] THEN
+  `∃m. n = SUC m` by (Cases_on `n` THEN FULL_SIMP_TAC (srw_ss()) []) THEN
+  SRW_TAC [][FUNPOW_SUC] THEN
+  SRW_TAC [][Once relationTheory.RTC_CASES1, normorder_rwts, lemma14b])
+
+val ceqnat_def = Define`
+  ceqnat = LAM "n"
+             (VAR "n" @@ cis_zero @@
+                (LAM "r" (LAM "m" (cand @@ (cnot @@ (cis_zero @@ (VAR "m"))) @@
+                                           (VAR "r" @@ (cpred @@ (VAR "m")))))))
+`;
+val FV_ceqnat = Store_thm(
+  "FV_ceqnat",
+  ``FV ceqnat = {}``,
+  SRW_TAC [][ceqnat_def, EXTENSION] THEN METIS_TAC []);
+
+val ceqnat_behaviour = store_thm(
+  "ceqnat_behaviour",
+  ``ceqnat @@ church n @@ church m -n->* cB (n = m)``,
+  SRW_TAC [][ceqnat_def, Once relationTheory.RTC_CASES1, normorder_rwts,
+             lemma14b] THEN DISJ2_TAC THEN
+  Q.MATCH_ABBREV_TAC
+      `church n @@ cis_zero @@ ff @@ church m -n->* cB(n = m)` THEN
+  SRW_TAC [][nstar_betastar_bnf] THEN
+  ONCE_REWRITE_TAC [relationTheory.RTC_CASES_RTC_TWICE] THEN
+  Q.EXISTS_TAC `FUNPOW ((@@) ff) n cis_zero @@ church m` THEN CONJ_TAC
+    THEN1 SRW_TAC [][betastar_APPl, nstar_betastar, church_behaviour] THEN
+  Q.ID_SPEC_TAC `m` THEN Induct_on `n` THENL [
+    ONCE_REWRITE_TAC [EQ_SYM_EQ] THEN
+    SRW_TAC [][nstar_betastar, cis_zero_behaviour],
+
+    ALL_TAC
+  ] THEN SRW_TAC [][FUNPOW_SUC] THEN
+  SRW_TAC [][Abbr`ff`, Once relationTheory.RTC_CASES1, GSYM nstar_betastar_bnf,
+             normorder_rwts, lemma14b] THEN DISJ2_TAC THEN
+  SRW_TAC [][Once relationTheory.RTC_CASES1, normorder_rwts, lemma14b] THEN
+  DISJ2_TAC THEN
+  `(m = 0) ∨ ∃m0. m = SUC m0` by (Cases_on `m` THEN SRW_TAC [][]) THEN
+  SRW_TAC [][] THENL [
+    SRW_TAC [][nstar_betastar_bnf] THEN
+    Q.MATCH_ABBREV_TAC
+        `cand @@ (cnot @@ (cis_zero @@ church 0)) @@ X -β->* cB F` THEN
+    ONCE_REWRITE_TAC [relationTheory.RTC_CASES_RTC_TWICE] THEN
+    Q.EXISTS_TAC `cand @@ cB F @@ X` THEN CONJ_TAC THENL [
+      ONCE_REWRITE_TAC [relationTheory.RTC_CASES_RTC_TWICE] THEN
+      Q.EXISTS_TAC `cand @@ (cnot @@ cB T) @@ X` THEN CONJ_TAC THENL [
+        MATCH_MP_TAC betastar_APPl THEN
+        MATCH_MP_TAC betastar_APPr THEN
+        MATCH_MP_TAC betastar_APPr THEN
+        MATCH_MP_TAC nstar_betastar THEN
+        ONCE_REWRITE_TAC [DECIDE ``T = (0 = 0)``] THEN
+        SRW_TAC [][cis_zero_behaviour],
+
+        MATCH_MP_TAC betastar_APPl THEN
+        MATCH_MP_TAC betastar_APPr THEN
+        MATCH_MP_TAC nstar_betastar THEN
+        ONCE_REWRITE_TAC [DECIDE ``F = ¬T``] THEN
+        SRW_TAC [][cnot_behaviour]
+      ],
+
+      SRW_TAC [][nstar_betastar, cand_F1]
+    ],
+
+    SRW_TAC [][nstar_betastar_bnf] THEN
+    Q.MATCH_ABBREV_TAC `cand @@ Cond1 @@ Cond2 -β->* cB bool` THEN
+    ONCE_REWRITE_TAC [relationTheory.RTC_CASES_RTC_TWICE] THEN
+    Q.EXISTS_TAC `cand @@ cB T @@ Cond2` THEN CONJ_TAC THENL [
+      MATCH_MP_TAC betastar_APPl THEN
+      MATCH_MP_TAC betastar_APPr THEN
+      SRW_TAC [][Abbr`Cond1`] THEN
+      Q.MATCH_ABBREV_TAC `cnot @@ Cond -β->* cB T` THEN
+      ONCE_REWRITE_TAC [relationTheory.RTC_CASES_RTC_TWICE] THEN
+      Q.EXISTS_TAC `cnot @@ cB F` THEN CONJ_TAC THENL [
+        SRW_TAC [][Abbr`Cond`] THEN
+        MATCH_MP_TAC betastar_APPr THEN
+        MATCH_MP_TAC nstar_betastar THEN
+        MATCH_ACCEPT_TAC
+            (SIMP_RULE (srw_ss()) [] (Q.INST [`n` |-> `SUC N`]
+                                             cis_zero_behaviour)),
+
+        MP_TAC (REWRITE_RULE [] (Q.INST [`p` |-> `F`] cnot_behaviour)) THEN
+        SRW_TAC [][nstar_betastar]
+      ],
+
+      ONCE_REWRITE_TAC [relationTheory.RTC_CASES_RTC_TWICE] THEN
+      Q.EXISTS_TAC `Cond2` THEN
+      SRW_TAC [][cand_T1, nstar_betastar] THEN
+      UNABBREV_ALL_TAC THEN
+      Q.MATCH_ABBREV_TAC `FF @@ Arg -β->* bool` THEN
+      ONCE_REWRITE_TAC [relationTheory.RTC_CASES_RTC_TWICE] THEN
+      Q.EXISTS_TAC `FF @@ church m0` THEN CONJ_TAC THEN1
+        SRW_TAC [][betastar_APPr, cpred_beta_SUC, Abbr`Arg`] THEN
+      SRW_TAC [][Abbr`bool`]
+    ]
+  ]);
+
 
 val _ = export_theory()
 
