examples/lambda/computability/churchboolScript.sml
@@ -10,6 +10,11 @@ val _ = new_theory "churchbool"
 
 val _ = set_trace "Unicode" 1
 
+val _ = remove_ovl_mapping "LAM" {Name="LAM", Thy="labelledTerms"}
+val _ = remove_ovl_mapping "FV"  {Name="FV",  Thy="labelledTerms"}
+val _ = remove_ovl_mapping "VAR" {Name="VAR", Thy="labelledTerms"}
+val _ = remove_ovl_mapping "@@"  {Name="APP", Thy="labelledTerms"}
+
 fun Store_thm(n,t,tac) = store_thm(n,t,tac) before export_rewrites [n]
 
 val cB_def = Define`cB p = LAM "x" (LAM "y" (VAR (if p then "x" else "y")))`;
@@ -20,6 +25,10 @@ val FV_cB = Store_thm(
 val bnf_cB = Store_thm(
   "bnf_cB",
   ``bnf (cB p)``,
+  SRW_TAC [][cB_def]);
+val cB_11 = Store_thm(
+  "cB_11",
+  ``(cB p = cB q) ⇔ (p ⇔ q)``,
   SRW_TAC [][cB_def]);
 
 val cB_behaviour = store_thm(
@@ -67,6 +76,23 @@ val cand_behaviour = store_thm(
              lemma14b] THEN
   SRW_TAC [][Once relationTheory.RTC_CASES1, normorder_rwts, lemma14b] THEN
   Cases_on `p` THEN SRW_TAC [][cB_behaviour]);
+
+val cand_F1 = store_thm(
+  "cand_F1",
+  ``cand @@ cB F @@ X -n->* cB F``,
+  SRW_TAC [][cand_def, Once relationTheory.RTC_CASES1, normorder_rwts,
+             lemma14b] THEN
+  SRW_TAC [][Once relationTheory.RTC_CASES1, normorder_rwts, lemma14b] THEN
+  SRW_TAC [][cB_behaviour]);
+
+val cand_T1 = store_thm(
+  "cand_T1",
+  ``cand @@ cB T @@ X -n->* X``,
+  SRW_TAC [][cand_def, Once relationTheory.RTC_CASES1, normorder_rwts,
+             lemma14b] THEN
+  SRW_TAC [][Once relationTheory.RTC_CASES1, normorder_rwts, lemma14b] THEN
+  SRW_TAC [][cB_behaviour]);
+
 
 val _ = export_theory()
 
