examples/lambda/computability/churchpairScript.sml
@@ -1,0 +1,75 @@
+open HolKernel boolLib bossLib Parse binderLib
+
+open chap3Theory
+open pred_setTheory
+open termTheory
+open boolSimps
+open normal_orderTheory
+open churchboolTheory
+
+val _ = new_theory "churchpair"
+
+val _ = set_trace "Unicode" 1
+
+fun Store_thm(n,t,tac) = store_thm(n,t,tac) before export_rewrites [n]
+val FUNPOW_SUC = arithmeticTheory.FUNPOW_SUC
+
+val cpair_def = Define`
+  cpair = LAM "x" (LAM "y" (LAM "f" (VAR "f" @@ VAR "x" @@ VAR "y")))
+`;
+
+val FV_cpair = Store_thm(
+  "FV_cpair",
+  ``FV cpair = {}``,
+  SRW_TAC [][cpair_def, EXTENSION] THEN METIS_TAC []);
+val bnf_cpair = Store_thm(
+  "bnf_cpair",
+  ``bnf cpair``,
+  SRW_TAC [][cpair_def]);
+
+val cfst_def = Define`
+  cfst = LAM "p" (VAR "p" @@ cB T)
+`;
+val FV_cfst = Store_thm(
+  "FV_cfst",
+  ``FV cfst = {}``,
+  SRW_TAC [][cfst_def])
+val bnf_cfst = Store_thm(
+  "bnf_cfst",
+  ``bnf cfst``,
+  SRW_TAC [][cfst_def]);
+
+val csnd_def = Define`
+  csnd = LAM "p" (VAR "p" @@ cB F)
+`;
+val FV_csnd = Store_thm(
+  "FV_csnd",
+  ``FV csnd = {}``,
+  SRW_TAC [][csnd_def])
+val bnf_csnd = Store_thm(
+  "bnf_csnd",
+  ``bnf csnd``,
+  SRW_TAC [][csnd_def]);
+
+val nstep_tac =
+    SRW_TAC [][Once relationTheory.RTC_CASES1, normorder_rwts, lemma14b]
+
+val cfst_pair = store_thm(
+  "cfst_pair",
+  ``cfst @@ (cpair @@ M @@ N) -n->* M``,
+  SRW_TAC [][cfst_def, cpair_def] THEN FRESH_TAC THEN SRW_TAC [][tpm_fresh] THEN
+  NTAC 3 (nstep_tac THEN DISJ2_TAC) THEN
+  SRW_TAC [][Once relationTheory.RTC_CASES1, normorder_rwts, lemma14b,
+             churchboolTheory.cB_behaviour]);
+
+val csnd_pair = store_thm(
+  "csnd_pair",
+  ``csnd @@ (cpair @@ M @@ N) -n->* N``,
+  SRW_TAC [][csnd_def, cpair_def] THEN FRESH_TAC THEN SRW_TAC [][tpm_fresh] THEN
+  NTAC 3 (nstep_tac THEN DISJ2_TAC) THEN
+  SRW_TAC [][Once relationTheory.RTC_CASES1, normorder_rwts, lemma14b,
+             churchboolTheory.cB_behaviour]);
+
+val _ = export_theory()
+
+
